src/Std/Data/DTreeMap/Raw/Iterator.lean
@@ -1,0 +1,53 @@
+/-
+Copyright (c) 2025 Lean FRO, LLC. All rights reserved.
+Released under Apache 2.0 license as described in the file LICENSE.
+Authors: Wojciech Różowski
+-/
+module
+
+prelude
+public import Std.Data.DTreeMap.Internal.Slice
+
+namespace Std.DTreeMap.Raw
+open Std.Iterators
+
+@[inline]
+public def iter {α : Type u} {β : α → Type v} [Ord α] (m : Raw α β) :=
+  (Internal.Zipper.iter_of_tree m.inner : Iter ((a : α) × β a))
+
+@[inline]
+public def keysIter {α : Type u} {β : α → Type u} [Ord α] (m : Raw α β) :=
+  (m.iter.map fun e => e.1 : Iter α)
+
+@[inline]
+public def valuesIter {α : Type u} {β : Type u} [Ord α](m : Raw α (fun _ => β)) :=
+  (m.iter.map fun e => e.2 : Iter β)
+
+public theorem iter_toList [Ord α] (m : Raw α β) :
+    m.iter.toList = m.toList := by
+  rw [Internal.toList_Zipper]
+  unfold iter
+  simp [Raw.toList]
+  rw [Internal.Zipper.iter_of_tree_toList_eq_zipper_prependMap_toList]
+
+public theorem keysIter_toList {α β} [Ord α] (m : Raw α β) :
+    m.keysIter.toList = m.keys := by
+  unfold keysIter
+  rw [Internal.toList_map_Zipper]
+  unfold iter
+  rw [Internal.iter_of_tree_internal_state_eq]
+  rw [Internal.Zipper.prependMap_done_toList_eq_toList]
+  unfold keys
+  simp [Internal.Impl.map_fst_toList_eq_keys]
+
+public theorem valuesIter_toList {α β} [Ord α] (m : Raw α (fun _ => β)) :
+    m.valuesIter.toList = m.values := by
+  unfold valuesIter
+  rw [Internal.toList_map_Zipper]
+  unfold iter
+  rw [Internal.iter_of_tree_internal_state_eq]
+  rw [Internal.Zipper.prependMap_done_toList_eq_toList]
+  unfold values
+  simp [Std.DTreeMap.Internal.Impl.values_eq_map_snd, Internal.Impl.toList_eq_toListModel]
+
+end Std.DTreeMap.Raw
